Relax bounds on literals during stringification
This results in fewer useless casts on literals, and fixes the
`to_bytes` Go synthesis issue.

The underlying assumption required by this change is that integer
literals don't need to be casted to be recognized as the narrowest
bitwidth that they fit into of the bitwidths we allow.  (This is
trivially true in C, at least.)

curve25519_64.c
@@ -94,16 +94,16 @@ static void fiat_25519_cmovznz_u64(uint64_t* out1, fiat_25519_uint1 arg1, uint64
  *   out1: [[0x0 ~> 0x8cccccccccccc], [0x0 ~> 0x8cccccccccccc], [0x0 ~> 0x8cccccccccccc], [0x0 ~> 0x8cccccccccccc], [0x0 ~> 0x8cccccccccccc]]
  */
 static void fiat_25519_carry_mul(uint64_t out1[5], const uint64_t arg1[5], const uint64_t arg2[5]) {
-  fiat_25519_uint128 x1 = ((fiat_25519_uint128)(arg1[4]) * ((arg2[4]) * (uint64_t)UINT8_C(0x13)));
-  fiat_25519_uint128 x2 = ((fiat_25519_uint128)(arg1[4]) * ((arg2[3]) * (uint64_t)UINT8_C(0x13)));
-  fiat_25519_uint128 x3 = ((fiat_25519_uint128)(arg1[4]) * ((arg2[2]) * (uint64_t)UINT8_C(0x13)));
-  fiat_25519_uint128 x4 = ((fiat_25519_uint128)(arg1[4]) * ((arg2[1]) * (uint64_t)UINT8_C(0x13)));
-  fiat_25519_uint128 x5 = ((fiat_25519_uint128)(arg1[3]) * ((arg2[4]) * (uint64_t)UINT8_C(0x13)));
-  fiat_25519_uint128 x6 = ((fiat_25519_uint128)(arg1[3]) * ((arg2[3]) * (uint64_t)UINT8_C(0x13)));
-  fiat_25519_uint128 x7 = ((fiat_25519_uint128)(arg1[3]) * ((arg2[2]) * (uint64_t)UINT8_C(0x13)));
-  fiat_25519_uint128 x8 = ((fiat_25519_uint128)(arg1[2]) * ((arg2[4]) * (uint64_t)UINT8_C(0x13)));
-  fiat_25519_uint128 x9 = ((fiat_25519_uint128)(arg1[2]) * ((arg2[3]) * (uint64_t)UINT8_C(0x13)));
-  fiat_25519_uint128 x10 = ((fiat_25519_uint128)(arg1[1]) * ((arg2[4]) * (uint64_t)UINT8_C(0x13)));
+  fiat_25519_uint128 x1 = ((fiat_25519_uint128)(arg1[4]) * ((arg2[4]) * UINT8_C(0x13)));
+  fiat_25519_uint128 x2 = ((fiat_25519_uint128)(arg1[4]) * ((arg2[3]) * UINT8_C(0x13)));
+  fiat_25519_uint128 x3 = ((fiat_25519_uint128)(arg1[4]) * ((arg2[2]) * UINT8_C(0x13)));
+  fiat_25519_uint128 x4 = ((fiat_25519_uint128)(arg1[4]) * ((arg2[1]) * UINT8_C(0x13)));
+  fiat_25519_uint128 x5 = ((fiat_25519_uint128)(arg1[3]) * ((arg2[4]) * UINT8_C(0x13)));
+  fiat_25519_uint128 x6 = ((fiat_25519_uint128)(arg1[3]) * ((arg2[3]) * UINT8_C(0x13)));
+  fiat_25519_uint128 x7 = ((fiat_25519_uint128)(arg1[3]) * ((arg2[2]) * UINT8_C(0x13)));
+  fiat_25519_uint128 x8 = ((fiat_25519_uint128)(arg1[2]) * ((arg2[4]) * UINT8_C(0x13)));
+  fiat_25519_uint128 x9 = ((fiat_25519_uint128)(arg1[2]) * ((arg2[3]) * UINT8_C(0x13)));
+  fiat_25519_uint128 x10 = ((fiat_25519_uint128)(arg1[1]) * ((arg2[4]) * UINT8_C(0x13)));
   fiat_25519_uint128 x11 = ((fiat_25519_uint128)(arg1[4]) * (arg2[0]));
   fiat_25519_uint128 x12 = ((fiat_25519_uint128)(arg1[3]) * (arg2[1]));
   fiat_25519_uint128 x13 = ((fiat_25519_uint128)(arg1[3]) * (arg2[0]));
@@ -138,7 +138,7 @@ static void fiat_25519_carry_mul(uint64_t out1[5], const uint64_t arg1[5], const
   fiat_25519_uint128 x42 = (x40 + x29);
   uint64_t x43 = (uint64_t)(x42 >> 51);
   uint64_t x44 = (uint64_t)(x42 & UINT64_C(0x7ffffffffffff));
-  uint64_t x45 = (x43 * (uint64_t)UINT8_C(0x13));
+  uint64_t x45 = (x43 * UINT8_C(0x13));
   uint64_t x46 = (x28 + x45);
   uint64_t x47 = (x46 >> 51);
   uint64_t x48 = (x46 & UINT64_C(0x7ffffffffffff));
@@ -164,14 +164,14 @@ static void fiat_25519_carry_mul(uint64_t out1[5], const uint64_t arg1[5], const
  *   out1: [[0x0 ~> 0x8cccccccccccc], [0x0 ~> 0x8cccccccccccc], [0x0 ~> 0x8cccccccccccc], [0x0 ~> 0x8cccccccccccc], [0x0 ~> 0x8cccccccccccc]]
  */
 static void fiat_25519_carry_square(uint64_t out1[5], const uint64_t arg1[5]) {
-  uint64_t x1 = ((arg1[4]) * (uint64_t)UINT8_C(0x13));
-  uint64_t x2 = (x1 * (uint64_t)0x2);
-  uint64_t x3 = ((arg1[4]) * (uint64_t)0x2);
-  uint64_t x4 = ((arg1[3]) * (uint64_t)UINT8_C(0x13));
-  uint64_t x5 = (x4 * (uint64_t)0x2);
-  uint64_t x6 = ((arg1[3]) * (uint64_t)0x2);
-  uint64_t x7 = ((arg1[2]) * (uint64_t)0x2);
-  uint64_t x8 = ((arg1[1]) * (uint64_t)0x2);
+  uint64_t x1 = ((arg1[4]) * UINT8_C(0x13));
+  uint64_t x2 = (x1 * 0x2);
+  uint64_t x3 = ((arg1[4]) * 0x2);
+  uint64_t x4 = ((arg1[3]) * UINT8_C(0x13));
+  uint64_t x5 = (x4 * 0x2);
+  uint64_t x6 = ((arg1[3]) * 0x2);
+  uint64_t x7 = ((arg1[2]) * 0x2);
+  uint64_t x8 = ((arg1[1]) * 0x2);
   fiat_25519_uint128 x9 = ((fiat_25519_uint128)(arg1[4]) * x1);
   fiat_25519_uint128 x10 = ((fiat_25519_uint128)(arg1[3]) * x2);
   fiat_25519_uint128 x11 = ((fiat_25519_uint128)(arg1[3]) * x4);
@@ -206,7 +206,7 @@ static void fiat_25519_carry_square(uint64_t out1[5], const uint64_t arg1[5]) {
   fiat_25519_uint128 x40 = (x38 + x27);
   uint64_t x41 = (uint64_t)(x40 >> 51);
   uint64_t x42 = (uint64_t)(x40 & UINT64_C(0x7ffffffffffff));
-  uint64_t x43 = (x41 * (uint64_t)UINT8_C(0x13));
+  uint64_t x43 = (x41 * UINT8_C(0x13));
   uint64_t x44 = (x26 + x43);
   uint64_t x45 = (x44 >> 51);
   uint64_t x46 = (x44 & UINT64_C(0x7ffffffffffff));
@@ -237,7 +237,7 @@ static void fiat_25519_carry(uint64_t out1[5], const uint64_t arg1[5]) {
   uint64_t x3 = ((x2 >> 51) + (arg1[2]));
   uint64_t x4 = ((x3 >> 51) + (arg1[3]));
   uint64_t x5 = ((x4 >> 51) + (arg1[4]));
-  uint64_t x6 = ((x1 & UINT64_C(0x7ffffffffffff)) + ((x5 >> 51) * (uint64_t)UINT8_C(0x13)));
+  uint64_t x6 = ((x1 & UINT64_C(0x7ffffffffffff)) + ((x5 >> 51) * UINT8_C(0x13)));
   uint64_t x7 = ((fiat_25519_uint1)(x6 >> 51) + (x2 & UINT64_C(0x7ffffffffffff)));
   uint64_t x8 = (x6 & UINT64_C(0x7ffffffffffff));
   uint64_t x9 = (x7 & UINT64_C(0x7ffffffffffff));
@@ -577,11 +577,11 @@ static void fiat_25519_from_bytes(uint64_t out1[5], const uint8_t arg1[32]) {
  *   out1: [[0x0 ~> 0x8cccccccccccc], [0x0 ~> 0x8cccccccccccc], [0x0 ~> 0x8cccccccccccc], [0x0 ~> 0x8cccccccccccc], [0x0 ~> 0x8cccccccccccc]]
  */
 static void fiat_25519_carry_scmul_121666(uint64_t out1[5], const uint64_t arg1[5]) {
-  fiat_25519_uint128 x1 = (UINT32_C(0x1db42) * (fiat_25519_uint128)(arg1[4]));
-  fiat_25519_uint128 x2 = (UINT32_C(0x1db42) * (fiat_25519_uint128)(arg1[3]));
-  fiat_25519_uint128 x3 = (UINT32_C(0x1db42) * (fiat_25519_uint128)(arg1[2]));
-  fiat_25519_uint128 x4 = (UINT32_C(0x1db42) * (fiat_25519_uint128)(arg1[1]));
-  fiat_25519_uint128 x5 = (UINT32_C(0x1db42) * (fiat_25519_uint128)(arg1[0]));
+  fiat_25519_uint128 x1 = ((fiat_25519_uint128)UINT32_C(0x1db42) * (arg1[4]));
+  fiat_25519_uint128 x2 = ((fiat_25519_uint128)UINT32_C(0x1db42) * (arg1[3]));
+  fiat_25519_uint128 x3 = ((fiat_25519_uint128)UINT32_C(0x1db42) * (arg1[2]));
+  fiat_25519_uint128 x4 = ((fiat_25519_uint128)UINT32_C(0x1db42) * (arg1[1]));
+  fiat_25519_uint128 x5 = ((fiat_25519_uint128)UINT32_C(0x1db42) * (arg1[0]));
   uint64_t x6 = (uint64_t)(x5 >> 51);
   uint64_t x7 = (uint64_t)(x5 & UINT64_C(0x7ffffffffffff));
   fiat_25519_uint128 x8 = (x6 + x4);
@@ -596,7 +596,7 @@ static void fiat_25519_carry_scmul_121666(uint64_t out1[5], const uint64_t arg1[
   fiat_25519_uint128 x17 = (x15 + x1);
   uint64_t x18 = (uint64_t)(x17 >> 51);
   uint64_t x19 = (uint64_t)(x17 & UINT64_C(0x7ffffffffffff));
-  uint64_t x20 = (x18 * (uint64_t)UINT8_C(0x13));
+  uint64_t x20 = (x18 * UINT8_C(0x13));
   uint64_t x21 = (x7 + x20);
   fiat_25519_uint1 x22 = (fiat_25519_uint1)(x21 >> 51);
   uint64_t x23 = (x21 & UINT64_C(0x7ffffffffffff));
